WIP: refactor: move assumptions to a typeclass instead of axioms
This PR introduces the `Language` typeclass, which subsumes some (but not yet all) axioms in which we encoded our assumptions.

EffectSSA/ProofSketch/InstSeq.lean
@@ -1,15 +1,19 @@
 module
 
-public import EffectSSA.ProofSketch.Inst
 public import EffectSSA.ProofSketch.VarSet
+public import EffectSSA.ProofSketch.Language
 
 /-!
 # Instruction Sequence
 -/
 namespace EffectSSA.ProofSketch
 open VarSet
+open Language (iArgs iResults)
 
-@[expose] public abbrev InstSeq := List Inst
+variable {ι Var Val State} [Language ι Var Val State]
+
+variable (ι) in
+@[expose] public abbrev InstSeq := List ι
 
 namespace InstSeq
 
@@ -18,13 +22,12 @@ namespace InstSeq
 -/
 noncomputable section Vars
 
-@[grind]
-def argsResults : InstSeq → VarSet × VarSet := go ∅ ∅
-where go (A R : VarSet)
+@[grind] def argsResults : InstSeq ι → VarSet Var × VarSet Var := go ∅ ∅
+where go (A R : VarSet Var)
   | [] => (A, R)
   | i :: is =>
-    let A := A ∪ (i.args - R)
-    let R := R ∪ i.results
+    let A := A ∪ (iArgs i - R)
+    let R := R ∪ iResults i
     go A R is
 
 /--
@@ -33,27 +36,27 @@ where go (A R : VarSet)
 Note: "free" means that any argument of an instruction `i ∈ is` that is also the
 result of any preceding instructions are *not* included in `is.args`.
 -/
-public def args (is : InstSeq) : VarSet :=
+public def args (is : InstSeq ι) : VarSet Var :=
   is.argsResults.1
 
 /-- `is.results` is the set of all results of sequence `is`. -/
-public def results (is : InstSeq) : VarSet :=
+public def results (is : InstSeq ι) : VarSet Var :=
   is.argsResults.2
 
 section Lemmas
-variable {i : Inst} {is : InstSeq}
+variable {i : ι} {is : InstSeq ι}
 attribute [local grind] results args argsResults argsResults.go
 
-@[grind =] theorem argsResults_go_fst (A R : VarSet) :
+@[grind =] theorem argsResults_go_fst (A R : VarSet Var) :
     (argsResults.go A R is).1 = A ∪ (args is - R) := by
   suffices ∀ A' R',
     (argsResults.go (A ∪ (A' - R)) (R ∪ R') is).fst = A ∪ ((argsResults.go A' R' is).fst - R)
   by simp [args, argsResults]; grind
   induction is generalizing A R <;> grind
 
-@[simp, grind =] public theorem args_nil : args [] = ∅ := by rfl
+@[simp, grind =] public theorem args_nil : args ([] : InstSeq ι) = ∅ := by rfl
 @[simp, grind =] public theorem args_cons :
-    args (i :: is) = i.args ∪ (args is - i.results) := by
+    args (i :: is) = iArgs i ∪ (is.args - iResults i) := by
   show (argsResults.go ..).fst = _; grind
 
 @[grind =] theorem argsResults_go_snd : (argsResults.go A R is).2 = R ∪ is.results := by
@@ -62,32 +65,32 @@ attribute [local grind] results args argsResults argsResults.go
   by simp [results, argsResults]; grind
   induction is generalizing A R <;> grind
 
-@[simp, grind =] public theorem results_nil  : results [] = ∅ := by rfl
-@[simp, grind =] public theorem results_cons : results (i :: is) = i.results ∪ is.results := by
+@[simp, grind =] public theorem results_nil  : results ([] : InstSeq ι) = ∅ := by rfl
+@[simp, grind =] public theorem results_cons : results (i :: is) = iResults i ∪ is.results := by
   show (argsResults.go ..).snd = _; grind
 
-@[simp, grind =] public theorem results_append {xs ys : InstSeq} :
+@[simp, grind =] public theorem results_append {xs ys : InstSeq ι} :
     results (xs ++ ys) = xs.results ∪ ys.results := by
   induction xs <;> grind
 
-@[grind =] public theorem mem_results_iff : x ∈ is.results ↔ ∃ i ∈ is, x ∈ i.results := by
+@[grind =] public theorem mem_results_iff : x ∈ is.results ↔ ∃ i ∈ is, x ∈ iResults i := by
   induction is <;> grind
 
-@[grind →] public theorem mem_results_of_mem_inst {x : Var} (hi : i ∈ is) (hx : x ∈ i.results) :
+@[grind →] public theorem mem_results_of_mem_inst {x : Var} (hi : i ∈ is) (hx : x ∈ iResults i) :
     x ∈ is.results := by
   grind
 
-@[grind →] public theorem results_subset_of_mem (h : i ∈ is) : i.results ⊆ is.results := by
+@[grind →] public theorem results_subset_of_mem (h : i ∈ is) : iResults i ⊆ is.results := by
   grind
 
 /--
 Recall that `is.args` contains only the *free* arguments of `is`, hence, for some `i ∈ is`,
-in general `i.args ⊈ is.args`. Instead, an argument `x ∈ i.args` might either be
+in general `args i ⊈ is.args`. Instead, an argument `x ∈ args i` might either be
 free (thus in `is.args`), or might refer to the result of an earlier instruction;
 the latter we over-approximate by the results of all instructions (`is.results`)
 -/
 @[grind →] public theorem args_subset_of_mem (h : i ∈ is) :
-    i.args ⊆ is.args ∪ is.results := by
+    iArgs i ⊆ is.args ∪ is.results := by
   induction is <;> grind
 
 end Lemmas
@@ -95,45 +98,45 @@ end Lemmas
 /-! ### getDef / usesAt  -/
 
 /--
-`is.getDef? v` returns an instruction `i ∈ is` s.t. `v ∈ i.results`,
+`is.getDef? v` returns an instruction `i ∈ is` s.t. `v ∈ iResults i`,
 or `none` if no such instruction exists
 -/
-public noncomputable def getDef? (v : Var) : (is : InstSeq) → Option { i // i ∈ is ∧ v ∈ is.results }
+public noncomputable def getDef? (v : Var) : (is : InstSeq ι) → Option { i // i ∈ is ∧ v ∈ is.results }
   | [] => none
   | i :: is =>
       open Classical in
-      if hi : v ∈ i.results then
+      if hi : v ∈ iResults i then
         some ⟨i, by grind⟩
       else
         (getDef? v is).map (fun ⟨i, hi⟩ => ⟨i, by grind⟩)
 
 /-- `is.UsesAt y x` is true when `y` is a (transitive) dependency of `x`. -/
 @[grind cases]
-public inductive UsesAt (is : InstSeq) (y : Var) : Var → Prop
-  | arg  : i ∈ is → x ∈ i.results → y ∈ i.args → UsesAt is y x
-  | trans : i ∈ is → x ∈ i.results → z ∈ i.args → UsesAt is y z → UsesAt is y x
+public inductive UsesAt (is : InstSeq ι) (y : Var) : Var → Prop
+  | arg  : i ∈ is → x ∈ iResults i → y ∈ iArgs i → UsesAt is y x
+  | trans : i ∈ is → x ∈ iResults i → z ∈ iArgs i → UsesAt is y z → UsesAt is y x
 
 /--
 `is.usesAt v` is the set of all transitive arguments that are used to compute
 variable `v`.
 
 That is, if `v` is defined by instruction `i ∈ is`, then `is.usesAt v` is the
-union of `i.args` with the recursive set `{ is.usesAt y | y ∈ i.args }`.
+union of `args i` with the recursive set `{ is.usesAt y | y ∈ args i }`.
 
 If no instruction of `is` defines the variable `v` as a result,
 then `is.usesAt v` is the empty set.
 -/
-public def usesAt (x : Var) (is : InstSeq) : VarSet :=
+public def usesAt (x : Var) (is : InstSeq ι) : VarSet Var :=
   { y | is.UsesAt y x }
 
 section Lemmas
-variable {is : InstSeq}
+variable {is : InstSeq ι}
 
 @[simp, grind =] public theorem mem_usesAt : y ∈ is.usesAt x ↔ is.UsesAt y x := by
   simp [usesAt]
 
 public theorem mem_usesAt' :
-    y ∈ is.usesAt x ↔ ∃ i ∈ is, x ∈ i.results ∧ (y ∈ i.args ∨ ∃ z ∈ i.args, y ∈ is.usesAt z) := by
+    y ∈ is.usesAt x ↔ ∃ i ∈ is, x ∈ iResults i ∧ (y ∈ iArgs i ∨ ∃ z ∈ iArgs i, y ∈ is.usesAt z) := by
   constructor
   · grind
   · simp only [mem_usesAt, forall_exists_index, and_imp]
@@ -141,8 +144,8 @@ public theorem mem_usesAt' :
     · apply UsesAt.arg hi hxi hy
     · apply UsesAt.trans hi hxi hzi hyz
 
-@[simp, grind .] public theorem not_usesAt_nil : ¬(UsesAt [] y x) := by grind
-@[simp, grind =] public theorem usesAt_nil_eq : usesAt x [] = ∅ := by grind
+@[simp, grind .] public theorem not_usesAt_nil : ¬(UsesAt ([] : InstSeq ι) y x) := by grind
+@[simp, grind =] public theorem usesAt_nil_eq : usesAt x ([] : InstSeq ι) = ∅ := by grind
 
 @[simp, grind =>]
 public theorem usesAt_eq_of_not_mem_results {x : Var} (h : x ∉ is.results) :
@@ -166,7 +169,7 @@ index into the sequence), as well as a way to index into the sequence with
 a PC.
 -/
 public section PC
-variable {is js : InstSeq}
+variable {is js : InstSeq ι}
 
 /--
 `is.PC` is the type of program counters of the sequence `is`.
@@ -174,7 +177,7 @@ variable {is js : InstSeq}
 Each program counter `pc : is.PC` uniquely identifies a location of the program.
 -/
 @[grind cases, grind]
-structure PC (is : InstSeq) : Type where
+structure PC (is : InstSeq ι) : Type where
   idx : Nat
   isLt : idx < is.length := by grind
 
@@ -183,7 +186,13 @@ structure PC (is : InstSeq) : Type where
   isLt := i.isLt
 
 /-- Get the instruction at the specified location. -/
-@[expose] def PC.get (pc : is.PC) : Inst := is[pc.idx]'pc.isLt
+@[expose] def PC.get (pc : is.PC) : ι := is[pc.idx]'pc.isLt
+
+@[expose, inherit_doc Language.iArgs]
+abbrev PC.args (pc : is.PC) : VarSet Var := iResults pc.get
+
+@[expose, inherit_doc Language.iResults]
+abbrev PC.results (pc : is.PC) : VarSet Var := iResults pc.get
 
 section Lemmas
 
@@ -209,16 +218,17 @@ namespace PC
     i.idx = j.idx → i = j := by grind
 
 /-! cases principle -/
+variable {i : ι} {is : InstSeq ι}
 
-@[grind] def zero {i is} : PC (i :: is) where idx := 0
-@[grind] def succ {i is} (p : PC is) : PC (i :: is) where idx := p.idx + 1
+@[grind] def zero : PC (i :: is) where idx := 0
+@[grind] def succ (p : PC is) : PC (i :: is) where idx := p.idx + 1
 
-@[grind =, simp] theorem get_zero : (@zero i is).get = i := by rfl
+@[grind =, simp] theorem get_zero : (@zero _ i is).get = i := by rfl
 @[grind =, simp] theorem get_succ (p : PC is) :
-    (@p.succ i _).get (is := no_index _) = p.get := by rfl
+    (@p.succ _ i _).get (is := no_index _) = p.get := by rfl
 
 @[grind =, simp] theorem succ_eq_succ_iff {p q : is.PC} :
-    (@p.succ i is) = q.succ ↔ p = q := by grind
+    (@p.succ _ i is) = q.succ ↔ p = q := by grind
 
 @[cases_eliminator, elab_as_elim]
 def consCases {motive : PC (i :: is) → Prop}
@@ -230,27 +240,27 @@ def consCases {motive : PC (i :: is) → Prop}
   case succ n => apply cast ?_ (succ ⟨n, by grind⟩); grind
 
 /-! append -/
-variable {is js : InstSeq}
+variable {is js : InstSeq ι}
 
 def appendLeft (p : PC is) : PC (is ++ js) where idx := p.idx
 def appendRight (p : PC js) : PC (is ++ js) where idx := p.idx + is.length
 
-@[grind =, simp] theorem idx_appendLeft :
-    (@appendLeft is js p).idx = p.idx := by rfl
+@[grind =, simp] theorem idx_appendLeft {p : PC is} :
+    (@p.appendLeft _ is js).idx = p.idx := by rfl
 
-@[grind =, simp] theorem idx_appendRight :
-    (@appendRight is js p).idx = p.idx + is.length := by rfl
+@[grind =, simp] theorem idx_appendRight {p : PC js} :
+    (@p.appendRight _ is js).idx = p.idx + is.length := by rfl
 
 @[grind =, simp] theorem get_appendLeft {p : PC is} :
-    (@appendLeft is js p).get = p.get := by grind [get]
+    (@p.appendLeft _ is js).get = p.get := by grind [get]
 
 @[grind =, simp] theorem get_appendRight {p : PC js} :
-    (@appendRight is js p).get = p.get := by grind [get]
+    (@p.appendRight _ is js).get = p.get := by grind [get]
 
 @[grind =, simp] theorem appendLeft_eq_appendLeft_iff (p q : PC is) :
-    (@p.appendLeft is js) = q.appendLeft ↔ p = q := by grind [appendLeft]
+    (@p.appendLeft _ is js) = q.appendLeft ↔ p = q := by grind [appendLeft]
 @[grind =, simp] theorem appendRight_eq_appendRight_iff (p q : PC js) :
-    (@p.appendRight is js) = q.appendRight ↔ p = q := by grind [appendRight]
+    (@p.appendRight _ is js) = q.appendRight ↔ p = q := by grind [appendRight]
 @[grind ., simp] theorem appendLeft_neq_appendRight (p : PC is) (q : PC js) :
     p.appendLeft ≠ q.appendRight := by grind [appendLeft, appendRight]
 
@@ -274,7 +284,7 @@ end Lemmas
 
 /-! Map PCs of `is` or `js` into `is ++ js`. -/
 section OfAppend
-variable {is js : InstSeq}
+variable {is js : InstSeq ι}
 
 public def PC.ofAppendLeft : is.PC → (is ++ js).PC
   | ⟨idx, isLt⟩ => ⟨idx, by grind⟩
@@ -284,12 +294,12 @@ public def PC.ofAppendRight : js.PC → (is ++ js).PC
 
 section AppendLemmas
 
-@[simp, grind =] public theorem get_ofAppendLeft :
-    (@PC.ofAppendLeft is js p).get = p.get := by
+@[simp, grind =] public theorem get_ofAppendLeft {p : PC _} :
+    (@p.ofAppendLeft _ is js).get = p.get := by
   grind [PC.get, PC.ofAppendLeft]
 
-@[simp, grind =] public theorem get_ofAppendRight :
-    (@PC.ofAppendRight is js p).get = p.get := by
+@[simp, grind =] public theorem get_ofAppendRight {p : PC _} :
+    (@p.ofAppendRight _ is js).get = p.get := by
   grind [PC.get, PC.ofAppendRight]
 
 end AppendLemmas
@@ -305,13 +315,13 @@ program in another.
 -/
 public section Embed
 
-structure EmbedIn (is js : InstSeq) where
+structure EmbedIn (is js : InstSeq ι) where
   map : is.PC → js.PC
   get_map : ∀ i, (map i).get = i.get
-  inj : ∀ i j : is.PC, i ≠ j → i.get.results ≠ ∅ → j.get.results ≠ ∅ → map i ≠ map j
+  inj : ∀ i j : is.PC, i ≠ j → i.results ≠ ∅ → j.results ≠ ∅ → map i ≠ map j
 
 -- `f : is.EmbedIn js` can be used a function
-instance {is js : InstSeq} : CoeFun (is.EmbedIn js) (fun _ => is.PC → js.PC) where
+instance {is js : InstSeq ι} : CoeFun (is.EmbedIn js) (fun _ => is.PC → js.PC) where
   coe f := f.map
 
 section Lemmas
@@ -343,10 +353,10 @@ public section WellFormed
 `is.NoShadowing` holds if no two instructions in `is` define the same
 resulting variable.
 -/
-inductive NoShadowing : InstSeq → Prop
+inductive NoShadowing : InstSeq ι → Prop
   | nil : NoShadowing []
-  | cons {i : Inst} {is : InstSeq} :
-      i.results.Disjoint is.results → NoShadowing is
+  | cons {i : ι} {is : InstSeq ι} :
+      (iResults i).Disjoint is.results → NoShadowing is
       → NoShadowing (i :: is)
 
 /--
@@ -357,13 +367,13 @@ A sequence `is` is well-formed, w.r.t. free variables `Γ`, when
 * `Γ` does not contain any result of `is`.
 -/
 @[grind, grind cases]
-structure WellFormed (Γ : VarSet) (is : InstSeq)  where
+structure WellFormed (Γ : VarSet Var) (is : InstSeq ι)  where
   noShadowing : is.NoShadowing
   args : is.args ⊆ Γ
   results : is.results.Disjoint Γ
 
 section Lemmas
-variable {is js : InstSeq}
+variable {is js : InstSeq ι}
 
 /-! ### Grind Annotations -/
 section Grind
@@ -378,18 +388,18 @@ end Grind
 section Basic
 attribute [local grind] WellFormed NoShadowing
 
-@[grind ., simp] theorem noShadowing_nil : NoShadowing [] := by grind
+@[grind ., simp] theorem noShadowing_nil : NoShadowing ([] : InstSeq ι) := by grind
 @[grind =, simp] theorem noShadowing_cons :
-    NoShadowing (i :: is) ↔ i.results.Disjoint is.results ∧ NoShadowing is := by grind
+    NoShadowing (i :: is) ↔ (iResults i).Disjoint is.results ∧ NoShadowing is := by grind
 
 @[grind =, simp] theorem noShadowing_append :
     NoShadowing (is ++ js) ↔ is.results.Disjoint js.results ∧ is.NoShadowing ∧ js.NoShadowing := by
   induction is <;> grind
 
-@[grind ., simp] theorem wellFormed_nil : WellFormed Γ [] := by grind
+@[grind ., simp] theorem wellFormed_nil : WellFormed Γ ([] : InstSeq ι) := by grind
 @[grind =, simp] theorem wellFormed_cons :
     WellFormed Γ (i :: is) ↔
-      i.args ⊆ Γ ∧ Γ.Disjoint i.results ∧ is.WellFormed (i.results ∪ Γ) := by
+      iArgs i ⊆ Γ ∧ Γ.Disjoint (iResults i) ∧ is.WellFormed (iResults i ∪ Γ) := by
   constructor
   · rintro ⟨⟩
     and_intros
@@ -414,11 +424,11 @@ section PC
 
 theorem noShadowing_iff :
     is.NoShadowing ↔ ∀ (i j : is.PC), i ≠ j →
-      i.get.results.Disjoint j.get.results := by
+      i.results.Disjoint j.results := by
   induction is
   case nil => grind
   case cons i is ih =>
-    change InstSeq at is
+    change InstSeq _ at is
     simp only [noShadowing_cons, ne_eq]
     constructor
     · rintro ⟨hdj, hns⟩
@@ -426,11 +436,11 @@ theorem noShadowing_iff :
       cases j <;> cases k <;> grind
     · intro h
       and_intros
-      · suffices ∀ j ∈ is, i.results.Disjoint j.results by grind
-        suffices ∀ j : is.PC, i.results.Disjoint j.get.results by grind
+      · suffices ∀ j ∈ is, (iResults i).Disjoint (iResults j) by grind
+        suffices ∀ j : is.PC, (iResults i).Disjoint j.results by grind
         intro j
         simpa using h .zero j.succ (by grind)
-      · suffices ∀ (i j : is.PC), i ≠ j → i.get.results.Disjoint j.get.results by grind
+      · suffices ∀ (i j : is.PC), i ≠ j → i.results.Disjoint j.results by grind
         intro j k hjk
         simpa using h j.succ k.succ (by grind)
 
@@ -441,15 +451,15 @@ section ResultLemmas
 
 @[grind <=]
 theorem results_disjoint_of_mem_of_noShadowing (hi : i ∈ is) (hj : j ∈ is) (wf : is.NoShadowing) :
-    i ≠ j → i.results.Disjoint j.results := by
+    i ≠ j → (iResults i).Disjoint (iResults j) := by
   induction is <;> grind
 
-theorem eq_of_not_disjoint_results_of_noShadowing {i j : Inst}
+theorem eq_of_not_disjoint_results_of_noShadowing {i j : ι}
     (hi : i ∈ is) (hj : j ∈ is) (wf : is.NoShadowing) :
-    ¬(i.results.Disjoint j.results) → i = j := by
+    ¬((iResults i).Disjoint (iResults j)) → i = j := by
   induction is <;> grind
 grind_pattern eq_of_not_disjoint_results_of_noShadowing =>
-  i.results.Disjoint j.results, i ∈ is, j ∈ is, is.NoShadowing
+  (iResults i).Disjoint (iResults j), i ∈ is, j ∈ is, is.NoShadowing
   -- ^^ TODO: this pattern seems overly specific, maybe I could drop the Disjoint pattern
 
 end ResultLemmas
