EffectSSA/ProofSketch/Language.lean
@@ -1,0 +1,75 @@
+module
+
+public import EffectSSA.ProofSketch.Denote
+public import EffectSSA.ProofSketch.VarSet
+
+/-!
+# Language Typeclass
+
+-/
+public section
+namespace EffectSSA.ProofSketch
+
+/-!
+## Environment
+We start by setting up the notion of the environment in which instructions will
+be denoted.
+-/
+section Env
+
+/--
+`PreLanguage` is an intermediate class in the construction of `Language`,
+with all the prerequites needed to define environments.
+
+Downstream users should *always* use `Language` directly.
+-/
+class PreLanguage (ι : Type) (Var Val State : outParam Type) where
+  /-- The initial (global) state that execution of a program starts with. -/
+  initialState : State
+
+/--
+An environment `ρ : Env ι` bundles a map from variables to values, with a global state.
+-/
+structure Env (ι) {Var Val State} [PreLanguage ι Var Val State] where
+  /-- A partial map from variables (i.e, virtual registers) to values. -/
+  regs : Var → Option Val := fun _ => none
+  /-- The global state, e.g, for memory and UB -/
+  state : State := PreLanguage.initialState ι
+  /--
+  Whether an interpreter error occured (e.g, a reference to an undefined
+  variable). This should never happen in well-formed programs.
+  -/
+  error : Bool := false
+
+end Env
+
+/-! ## Language Class -/
+/--
+`Language` bundles the basic assumptions that form a language in our setting:
+
+* `ι` is the type of instructions
+* `Var` is the type variable names
+* `Val` is the type of runtime values
+* `State` is the type of global state (e.g, memory)
+
+Besides these types, we ask for:
+
+* An initial global state,
+* A way to denote individual instructions as a map on (stateful) environments,
+* That equality of instructions is decidable,
+* A map from an instruction to its arguments, and
+* A map from an instruction to its results
+-/
+class Language (ι : Type) (Var Val State : outParam Type) extends
+    PreLanguage ι Var Val State,
+    Denote ι (Env ι → Env ι) where
+
+  /-- Equality of instructions must be decidable. -/
+  [decideInstEq : DecidableEq ι]
+
+  /-- `iArgs i` is the set of arguments of instruction `i`. -/
+  iArgs : ι → VarSet Var
+  /-- `iResults i` is the set of results of instruction `i`. -/
+  iResults : ι → VarSet Var
+
+attribute [reducible, instance] Language.decideInstEq
